basic_types0.v
@@ -1,0 +1,1008 @@
+(*Trivial facts that would clutter up the other files*) 
+Require Import ssreflect.
+From mathcomp Require Import ssreflect seq ssrnat.
+From istari Require Import Sigma Tactics
+     Syntax Subst SimpSub Promote Hygiene
+     ContextHygiene Equivalence Equivalences Rules Defined PageType lemmas0 derived_rules.
+Lemma subst_U0: forall s,
+    (@ subst obj s (univ nzero)) = univ nzero.
+  auto. Qed.
+Hint Rewrite subst_U0: core subst1.
+
+Lemma subst_nzero: forall s,
+    @ subst obj s nzero = nzero.
+  intros. unfold nzero. auto. Qed.
+Hint Rewrite subst_nzero: core subst1.
+Ltac simpsub1 :=
+autounfold with subst1; autorewrite with subst1.
+
+Ltac simpsub_big := repeat (simpsub; simpsub1).
+
+
+Hint Unfold subst1: subst1.
+
+Ltac var_solv0 := try (apply tr_hyp_tm; repeat constructor).
+ Lemma bool_contra G m n A : tr G (deq bfalse btrue booltp) ->
+                          tr G (deq m n A).
+   intros Hcontra. apply (tr_voidtp_elim _ triv triv).
+   eapply (tr_compute _ _ (bite btrue voidtp unittp)).
+   apply equiv_symm. apply reduce_equiv. apply reduce_bite_beta1.
+ apply reduce_id. apply equiv_refl. apply equiv_refl.
+ eapply tr_eqtype_convert. apply tr_booltp_elim_eqtype;
+                             try apply Hcontra;
+                             apply (tr_formation_weaken _ nzero). apply tr_voidtp_formation.
+ apply tr_unittp_formation.
+ eapply tr_compute. apply reduce_equiv. apply reduce_bite_beta2.
+ apply reduce_id. apply equiv_refl. apply equiv_refl.
+ constructor.
+Qed.
+
+ Lemma tr_wt_intro 
+    G a b m m' n n':
+      tr G (deq m m' a)
+      -> tr G (deq n n' (subst1 m (arrow b (subst sh1 (wt a b)))))
+      -> tr (cons (hyp_tm a) G) (deqtype b b)
+      -> tr G (deq (ppair m n) (ppair m' n') (wt a b)).
+ intros Hm Hn Hb.
+ apply (tr_subtype_elim _ (sigma a
+                                 (arrow b (subst sh1 (wt a b))))).
+ apply tr_wt_sigma_subtype.
+ {eapply tr_inhabitation_formation. apply Hm. }
+ {assumption. }
+ { apply tr_sigma_intro; try assumption.
+   apply tr_arrow_formation; try assumption.
+   rewrite make_app1 ! subst_sh_shift.
+   apply tr_weakening_appendt. apply tr_wt_formation.
+ eapply tr_inhabitation_formation. apply Hm. assumption.
+ } Qed.
+
+ Definition U0 : (term obj) := univ nzero.
+
+Lemma nat_U01 G: tr ((hyp_tm booltp)::G) (oof (bite (var 0) voidtp unittp) U0).
+change U0 with (subst1 (var 0) U0).
+apply tr_booltp_elim. change booltp with (@subst obj (sh 1) booltp). var_solv0. apply tr_voidtp_formation. apply tr_unittp_formation.
+Qed.
+
+
+Lemma nat_U0: forall G,
+    tr G (oof nattp U0).
+  intros. unfold nattp.
+  apply tr_wt_formation_univ. constructor.
+  change (univ (subst sh1 nzero)) with
+      (subst1 (var 0) U0).
+  apply tr_booltp_elim.
+  change booltp with (@subst obj sh1 booltp). var_solv0.
+  simpsub_big. apply tr_voidtp_formation.
+  simpsub_big. apply tr_unittp_formation. Qed.
+
+Hint Resolve nat_U0. 
+
+Lemma nat_type: forall G,
+    tr G (deqtype nattp nattp).
+  intros. eapply tr_formation_weaken. apply nat_U0. Qed.
+Hint Resolve nat_type. 
+
+Lemma unit_type: forall G,
+      tr G (deqtype unittp unittp). 
+  intros. eapply tr_formation_weaken. apply tr_unittp_formation. Qed.
+
+Hint Resolve unit_type. 
+
+Lemma bool_type: forall G,
+      tr G (deqtype booltp booltp). 
+  intros. eapply tr_formation_weaken. apply tr_booltp_formation. Qed.
+
+Hint Resolve bool_type.
+
+Lemma void_type: forall G,
+      tr G (deqtype voidtp voidtp). 
+  intros. eapply tr_formation_weaken. apply tr_voidtp_formation. Qed.
+
+Hint Resolve void_type.
+
+ Definition if_z (n: term obj): (term obj) := ppi1 n.
+
+
+Lemma zero_typed: forall G,
+    tr G (oof nzero nattp).
+  intros.  unfold nattp. unfold nzero.
+  apply tr_wt_intro. 
+  {constructor. }
+  {simpsub_big.  apply tr_arrow_intro; auto.
+   apply tr_booltp_elim_eqtype; auto. constructor.
+   eapply (tr_compute_hyp _ [::]). constructor.
+   {apply reduce_equiv. apply reduce_bite_beta1.
+    apply reduce_id. }
+   simpl.  apply (tr_voidtp_elim _ (var 0) (var 0)).
+   rewrite - (subst_voidtp obj (sh 1)). var_solv0.
+  }
+   apply tr_booltp_elim_eqtype; auto.  
+   rewrite - (subst_booltp obj (sh 1)). var_solv0. Qed.
+
+Hint Resolve zero_typed :core .
+
+Lemma U0_type: forall G,
+    tr G (deqtype U0 U0).
+  intros. apply tr_univ_formation; auto. Qed.
+
+Hint Resolve U0_type : core.
+
+Lemma subst_nat: forall s,
+    @ subst obj s nattp = nattp.
+  intros. unfold nattp. auto. Qed.
+
+Hint Rewrite subst_nat: core subst1.
+
+Definition lt_t n m : term obj :=
+  app (app lttp n) m.
+
+Definition leq_b n1 := app (wind (lam (* x = 0*)
+                             (lam (*x = 1, y= 0*)
+                                ( lam
+                                    ( (*x = 2, y = 1, z = 0*)
+                                      bite (var 2) (*if n1 = 0*)
+                                           (lam (*x = 3, y = 2, z = 1, n2 = 0*)
+                                             btrue) 
+                                           ( 
+                                             lam
+                                               ( (*x = 3, y = 2, z = 1, n2 = 0*)
+                                                 bite (if_z (var 0))
+                                                      bfalse
+                                                      (app (app (var 1) triv) (app (ppi2 (var 0)) triv))
+                                               )
+                                           )
+                                    )
+                                )
+                             )                           
+                            )) n1.
+Definition leqb_app n1 n2 := app (leq_b n1) n2.
+Definition ltb_app n1 n2 := app (leq_b (nsucc n1)) n2.
+
+
+
+Lemma equiv_equal :
+  forall (m m' n n' t t' : term obj),
+    equiv t t' ->
+    equiv m m'
+    -> equiv n n'
+    -> equiv (equal t m n) (equal t' m' n').
+Proof.
+prove_equiv_compat.
+Qed.
+
+
+
+Ltac weaken H := eapply tr_formation_weaken; apply H.
+
+Hint Rewrite subst_nat: core subst1.
+
+Ltac var_solv' := unfold oof; match goal with |- tr ?G' (deq (var ?n) ?n' ?T) =>
+                                              try rewrite - (subst_nat (sh (n.+1)));
+                                              try rewrite - (subst_unittp _ (sh (n.+1)));
+                                              try rewrite - (subst_arrow _ (sh (n.+1)));
+                                                                               var_solv0 end.
+
+Lemma equiv_arrow :
+  forall (m m' n n' : term obj),
+    equiv m m'
+    -> equiv n n'
+    -> equiv (arrow m n) (arrow m' n').
+Proof.
+prove_equiv_compat.
+Qed.
+
+
+Lemma nsucc_type G n m:
+  tr G (deq n m nattp) ->
+  tr G (deq (nsucc n) (nsucc m) nattp).
+  intros.  unfold nsucc.
+  apply tr_wt_intro.
+  constructor. simpsub_big.
+  apply tr_arrow_intro; try apply tr_booltp_elim_eqtype; auto. constructor.
+  rewrite ! subst_sh_shift make_app1. apply tr_weakening_append1. assumption.
+  apply tr_booltp_elim_eqtype; auto.
+  change  booltp with (@subst obj sh1 booltp). var_solv0. Qed.
+
+Hint Resolve nsucc_type. 
+
+Definition nat_ind_fn : (term obj) := lam (lam (lam (lam (*P = 3 BC = 2 IS = 1 x = 0 *)
+                                          (app (
+                                            wind ( lam (lam (lam ( (*c = 0, b= 1, a = 2, x = 3, IS = 4, BC = 5,
+                                                                    P = 6*)
+                                                                 bite (var 2) (var 5)
+                                                                      (app (app (var 4)
+                                                                           (app (var 1) triv))
+                                                                           (app (var 0) triv))
+                          )))))                
+                                               (var 0)
+                                          )
+                                               ))).
+
+Definition nat_elim G := (tr_wt_elim G booltp (bite (var 0) voidtp unittp)).
+
+
+
+Lemma w_elim_hyp G1 G2 a b J :
+  tr G1 (deqtype a a) ->
+      tr (cons (hyp_tm a) G1) (deqtype b b) ->
+      tr (G2 ++ hyp_tm (sigma a (arrow b (subst sh1 (wt a b)))) :: G1) J
+      -> tr (G2 ++ hyp_tm (wt a b) :: G1) J.
+  intros. eapply tr_subtype_convert_hyp; unfold dsubtype;
+  change triv with (@shift obj 1 triv);
+  change (subtype
+       (subst sh1 ?one)
+       (subst sh1 ?sigma)) with
+      (subst sh1 (subtype one sigma)) (*ask karl if i write shift here it doesnt work*); try rewrite ! subst_sh_shift;
+    try apply tr_weakening_append1. apply tr_wt_subtype_sigma; auto.
+  apply tr_wt_sigma_subtype; auto.
+  assumption.
+Qed.
+
+
+
+  Lemma nat_ind G : tr G (oof nat_ind_fn
+                              (pi (arrow nattp U0)
+                                  (pi (app (var 0) nzero)
+                                         (pi (pi nattp
+                                                    (
+                                                      arrow (app (var 2) (var 0))
+                                                            (app (var 2) (nsucc (var 0)))
+                                                           )
+                                                )
+                                                (pi nattp
+                                                    (app (var 3) (var 0))
+                                                )
+                                         )
+                                  )
+                         )).
+    intros.
+    assert (forall G2 x y, tr (G2 ++ (hyp_tm (arrow nattp U0) :: G))
+                       (deq x y nattp) ->
+        (tr (G2 ++ (hyp_tm (arrow nattp U0) :: G))
+            (deqtype (app (var (length G2)) x) (app (var (length G2)) y)))) as Hp.
+    intros.
+      eapply tr_formation_weaken. apply (tr_arrow_elim _ nattp); auto.
+      apply U0_type.
+change (arrow (nattp) (univ nzero)) with
+    (@subst obj (sh (length G2)) (arrow nattp (univ nzero))). change (var (length G2)) with (@subst obj (sh (length G2)) (var 0)). rewrite ! subst_sh_shift. apply tr_weakening_append.
+change (arrow (nattp) (univ nzero)) with
+    (@subst obj (sh 1) (arrow nattp (univ nzero))). var_solv0.
+    simpl.
+    apply tr_pi_intro. apply tr_arrow_formation; auto.
+    apply tr_pi_intro; auto.
+    + apply (Hp [::]); auto.
+  (*  + apply tr_arrow_formation; auto. apply tr_pi_formation; auto.
+      apply tr_arrow_formation; auto.
+      rewrite make_app1. eapply Hp; auto. simpl. var_solv'.
+      rewrite make_app1. eapply Hp; simpl; auto. apply nsucc_type. var_solv'.
+      apply tr_pi_formation; auto.
+      rewrite make_app1. eapply Hp; auto. simpl. var_solv'.*)
+    + apply tr_pi_intro; auto.
+      - apply tr_pi_formation; auto. apply tr_arrow_formation; auto.
+      rewrite make_app2. eapply Hp; auto. simpl. var_solv'.
+      rewrite make_app2. eapply Hp; simpl; auto. apply nsucc_type. var_solv'.
+      - apply tr_pi_intro; auto. change (app (var 3) (var 0)) with
+                                     (@subst1 obj (var 0) (app (var 4) (var 0))).
+        eapply nat_elim. fold (@nattp obj). var_solv'.
+        change (var 5) with (@subst obj (under 2 sh1) (var 4)).
+        change (app (app (var 4) (app (var 1) triv))
+                    (app (var 0) triv)) with (@subst obj (under 2 sh1)
+(app (app (var 3) (app (var 1) triv))
+                    (app (var 0) triv)) 
+                                             ).
+        rewrite make_app2. apply tr_booltp_eta_hyp. (*true case*) 
+        { repeat (simpl; simpsub). rewrite make_app1.
+          eapply tr_compute_hyp.
+        {
+          constructor. apply equiv_arrow. apply reduce_equiv.
+          apply reduce_bite_beta1. apply reduce_id.
+          apply equiv_refl.
+        }
+        simpl. eapply (tr_compute_hyp _ [::]).
+        {
+          constructor. apply equiv_pi. apply reduce_equiv.
+          apply reduce_bite_beta1. apply reduce_id.
+          apply equiv_refl.
+        }
+        simpl.
+        apply (tr_eqtype_convert _#3 (app (var 5) nzero)).
+        { 
+          rewrite make_app5. apply Hp.
+          unfold nzero. apply tr_wt_intro. constructor.
+          simpsub. eapply tr_compute.
+          apply equiv_arrow. apply reduce_equiv.
+          apply reduce_bite_beta1. apply reduce_id.
+          apply equiv_refl. apply equiv_refl. apply equiv_refl.
+          apply (tr_transitivity _ _ (lam (app (subst sh1 (var 1)) (var 0))) ).
+          {
+            simpsub. simpl. apply tr_arrow_intro; auto.
+            - 
+              apply (tr_voidtp_elim _ (var 0) (var 0)).
+              change voidtp with (@subst obj (sh 1) voidtp).
+              var_solv0.
+          }
+          apply tr_symmetry. apply tr_arrow_eta.
+          change 
+            (arrow voidtp nattp)
+            with (@subst obj (sh 2)
+            (arrow voidtp nattp)
+                 ). var_solv0.
+          apply tr_booltp_elim_eqtype. change booltp with (@subst obj (sh 1) booltp). var_solv0. weaken tr_voidtp_formation. weaken tr_unittp_formation. }
+        change (app (var 5) nzero) with
+            (@subst obj (sh 5) (app (var 0) nzero)). var_solv0. }
+        (*false case*)
+        { repeat (simpl; simpsub). rewrite make_app1.
+          eapply tr_compute_hyp.
+        {
+          constructor. apply equiv_arrow. apply reduce_equiv.
+          apply reduce_bite_beta2. apply reduce_id.
+          apply equiv_refl.
+        }
+        simpl. eapply (tr_compute_hyp _ [::]).
+        {
+          constructor. apply equiv_pi. apply reduce_equiv.
+          apply reduce_bite_beta2. apply reduce_id.
+          apply equiv_refl.
+        }
+        simpl.
+        apply (tr_eqtype_convert _#3 (app (var 5) (ppair bfalse
+                                                         (lam (app (var 2) triv))
+              ))).
+        rewrite make_app5. apply Hp. apply tr_wt_intro; auto. constructor.
+        (*b = \x.b * *)
+        {
+          simpsub.
+          eapply tr_compute. apply equiv_arrow.
+           apply reduce_equiv.
+           apply reduce_bite_beta2. apply reduce_id. apply equiv_refl. apply equiv_refl.
+           apply equiv_refl.
+          simpsub. simpl. 
+          apply (tr_transitivity _ _
+                                           (lam (app (var 2) (var 0)))
+                          ).
+          {
+            apply tr_arrow_intro; auto.
+            apply (tr_arrow_elim _ unittp); auto.
+            match goal with |- tr ?G (deq ?M ?M ?T) =>
+                                                      change T with
+       (@subst obj (sh 3)                                   
+       (arrow unittp
+          (wt booltp
+              (bite (var 0) voidtp unittp)))) end. var_solv0.
+          apply tr_symmetry. apply tr_unittp_eta.
+          change unittp with (@subst obj (sh 1) unittp). var_solv0.
+          }
+          {
+            apply tr_symmetry.
+            apply tr_arrow_eta.
+            match goal with |- tr ?G (deq ?M ?M ?T) =>
+                                                      change T with
+       (@subst obj (sh 2)                                   
+       (arrow unittp
+          (wt booltp
+              (bite (var 0) voidtp unittp)))) end. var_solv0.
+          }
+        }
+        weaken nat_U01.
+        (* IS (b triv ) (c triv) : P (succ (b triv )) *)
+        apply (tr_arrow_elim _ (app (var 5) (app (var 1) triv))).
+          * rewrite make_app5. apply Hp.
+            apply (tr_arrow_elim _ unittp); auto. 
+            change (arrow unittp nattp) with (@subst obj (sh 2)
+                                                     (arrow unittp nattp)).
+            var_solv0. constructor.
+            rewrite make_app5. apply Hp.
+            change (ppair bfalse (lam (app (var 2) triv))) with
+                (@nsucc obj (app (var 1) triv)).
+            apply nsucc_type.
+            apply (tr_arrow_elim _ unittp); auto.
+            change (arrow unittp nattp) with (@subst obj (sh 2)
+                                                     (arrow unittp nattp)).
+            var_solv0. constructor.
+            match goal with |- tr ?G (deq ?M ?M ?T) => change T with
+                (@subst1 obj (app (var 1) triv)
+                (arrow (app (var 6) (var 0))
+          (app (var 6)
+               (ppair bfalse (lam (var 1)))))
+                ) end.
+            apply (tr_pi_elim _ nattp).
+            match goal with |- tr ?G (deq ?M ?M ?T) => change T with
+                (@subst obj (sh 4)
+       (pi nattp
+          (arrow (app (var 2) (var 0))
+             (app (var 2)
+                  (ppair bfalse (lam (var 1))))))) end.
+            var_solv0.
+            apply (tr_arrow_elim _ unittp); auto.
+            change (arrow unittp nattp) with (@subst obj (sh 2)
+                                                     (arrow unittp nattp)).
+            var_solv0. constructor.
+            change (app (var 5) (app (var 1) triv)) with (@subst1 obj triv
+(app (var 6) (app (var 2) (var 0)))
+                                                         ).
+            apply (tr_pi_elim _ unittp). 
+            change (pi unittp (app (var 6) (app (var 2) (var 0))))
+              with (@subst obj (sh 1)
+(pi unittp (app (var 5) (app (var 1) (var 0))))
+                   ). var_solv0.
+            constructor. }
+            Qed.
+
+  Lemma nat_ind_app G P BC IS: tr G (oof P (arrow nattp U0)) ->
+                        tr G (oof BC (app P nzero)) ->
+                        tr G (oof IS
+                                  (pi nattp
+                                      (arrow (app (shift 1 P) (var 0))
+                                             (app (shift 1 P) (nsucc (var 0)))
+                                  ))) ->
+                              tr G (oof (app (app (app nat_ind_fn P) BC
+                                   ) IS)
+                                                (pi nattp
+                                                    (app (shift 1 P) (var 0))
+                                   )).
+    intros.
+    replace (pi nattp (app (shift 1 P) (var 0))) with
+        (subst1 IS
+(pi nattp (app (shift 2 P) (var 0)))
+        ).
+    2:{
+      rewrite - ! subst_sh_shift. simpsub. unfold subst1. auto.
+    }
+    apply (tr_pi_elim _
+           (pi nattp
+             (arrow (app (shift 1 P) (var 0))
+                      (app (shift 1 P) (nsucc (var 0))))
+          )).
+    match goal with |- tr ?G (deq ?T ?T ?A) =>
+                    replace A with
+        (subst1 BC
+       (pi
+          (pi nattp
+             (arrow (app (shift 2 P) (var 0))
+                (app (shift 2 P)
+                   (nsucc (var 0)))))
+          (pi nattp
+             (app (shift 3 P) (var 0))))) end.
+    2:{ unfold nsucc.
+      rewrite - ! subst_sh_shift. simpsub. unfold subst1. 
+      simpsub. auto.
+    }
+    apply (tr_pi_elim _ (app P nzero)).
+    match goal with |- tr ?G (deq ?T ?T ?A) =>
+                    replace A with (subst1 P
+       (pi (app (var 0) nzero)
+          (pi
+             (pi nattp
+                (arrow
+                   (app (var 2)
+                      (var 0))
+                   (app (var 2)
+                      (nsucc (var 0)))))
+             (pi nattp
+                 (app (var 3) (var 0)))))) end.
+    eapply tr_pi_elim; try apply nat_ind; auto.
+    unfold nsucc. unfold nzero. simpsub. rewrite - ! subst_sh_shift. simpl.
+    auto. assumption. assumption.
+  Qed.
+
+
+Hint Rewrite <- subst_sh_shift: core subst1.
+
+  Lemma nat_ind_lamapp G P BC IS IS_type: tr G (oof (lam P) (arrow nattp U0)) ->
+                                  tr G (oof BC (subst1 nzero P)) ->
+                                  IS_type = (subst1 (nsucc (var 0)) (subst (under 1 (sh 1)) P)) ->
+                        tr G (oof IS
+                                  (pi nattp
+                                      (arrow P IS_type
+                                             
+                                  ))) ->
+                              tr G (oof (app (app (app nat_ind_fn (lam P)) BC
+                                   ) IS)
+                                                (pi nattp
+                                                    P)).
+    intros.
+    -
+      replace P with (subst1 (var 0) (subst (under 1 (sh 1)) P)) at 2.
+      2:{ simpsub_big. auto. rewrite - {2} (subst_id obj P).
+          apply subst_eqsub. apply eqsub_symm. apply eqsub_expand_id. }
+      eapply tr_compute.
+apply equiv_symm. apply equiv_pi. apply equiv_refl.
+apply reduce_equiv. apply reduce_app_beta; apply reduce_id.
+apply equiv_refl. apply equiv_refl.
+rewrite - subst_lam subst_sh_shift.
+apply nat_ind_app; try assumption.
+    - eapply tr_compute.  apply reduce_equiv; try apply reduce_app_beta;
+                            apply reduce_id. apply equiv_refl. apply equiv_refl. assumption.
+    - eapply tr_compute. apply equiv_pi. apply equiv_refl.
+      apply equiv_arrow; rewrite - subst_sh_shift subst_lam; apply reduce_equiv; apply reduce_app_beta; apply reduce_id. apply equiv_refl. apply equiv_refl.
+      replace (subst1 (var 0) (subst (under 1 (sh 1)) P)) with P.
+      2:{ simpsub_big. auto. rewrite - {1}  (subst_id obj P).
+          apply subst_eqsub. apply eqsub_expand_id. }
+      subst. assumption.
+Qed.
+
+
+Definition leq_t n m : term obj :=
+  app (app leqtp n) m.
+
+Lemma leq_type: forall G n1 n2,
+    tr G (oof n1 nattp) -> tr G (oof n2 nattp) ->
+    tr G (oof (leq_t n1 n2) U0).
+  intros. unfold leq_t.
+  apply (tr_arrow_elim _ nattp); auto.
+  unfold leqtp.
+  change (arrow nattp U0) with (subst1 n1 (arrow nattp U0)).
+  apply (tr_wt_elim _ booltp (bite (var 0) voidtp unittp)).
+  - assumption.
+  - simpsub. simpl.
+    rewrite make_app2.
+     change (lam unittp) with
+      (@subst obj (under 2 sh1)  (lam unittp)) .
+    change 
+          (lam
+             (bite (ppi1 (var 0)) voidtp
+                (app (app (var 1) triv)
+                   (app (ppi2 (var 0)) triv))))
+ with
+        (@subst obj (under 2 sh1)
+          (lam
+             (bite (ppi1 (var 0)) voidtp
+                (app (app (var 1) triv)
+                   (app (ppi2 (var 0)) triv))))).
+    apply tr_booltp_eta_hyp; simpsub; simpl; simpsub;
+    (*rewrite ! subst_nat; *)
+      apply tr_arrow_intro; auto; try weaken tr_booltp_formation.
+    {simpsub_big. apply tr_unittp_formation. }
+    + simpsub_big. apply (w_elim_hyp _ [::]); auto.
+      weaken nat_U01.
+      match goal with |- tr ?G (deq ?M ?M ?A) => change M with
+       (@subst obj (under 0 (dot (ppi2 (var 0)) (dot (ppi1 (var 0)) sh1)))
+       (bite (var 1) voidtp
+          (app (app (var 2) triv)
+               (app (var 0) triv)))) end.
+      apply tr_sigma_eta_hyp.
+      simpsub_big. simpl.
+          change (app (app (var 2) triv)
+                      (app (var 0) triv)) with
+              (@subst obj (under 1 sh1)
+                     (app (app (var 1) triv)
+                          (app (var 0) triv))).
+          change voidtp with (@subst obj (under 1 sh1) voidtp).
+          rewrite make_app1.
+          apply tr_booltp_eta_hyp; simpsub_big; auto.
+      * apply tr_voidtp_formation. 
+      * eapply tr_compute_hyp.
+        {
+          constructor. apply equiv_pi. apply reduce_equiv.
+          apply reduce_bite_beta2. apply reduce_id.
+          apply equiv_refl.
+        }
+        simpl. eapply (tr_compute_hyp _ [::]).
+        {
+          constructor. apply equiv_arrow. apply reduce_equiv.
+          apply reduce_bite_beta2. apply reduce_id.
+          apply equiv_refl.
+        }
+        simpl.
+        apply (tr_arrow_elim _ nattp); auto.  
+        change (arrow nattp (univ nzero)) with
+            (@subst1 obj triv (arrow nattp (univ nzero))).
+        apply (tr_pi_elim _ (unittp)).
+        - change (pi unittp (arrow nattp (univ nzero)))
+          with (@subst obj (sh 2) (pi unittp (arrow nattp (univ nzero)))).
+        var_solv0. constructor.
+        - apply (tr_arrow_elim _ unittp); auto. 
+          change (arrow unittp nattp) with (@subst obj (sh 1) (arrow
+                                                                 unittp nattp)).
+          var_solv0.
+          constructor.
+Qed.
+
+
+Lemma leq_succ_equiv n1_pred n2 : equiv (leq_t (ppair bfalse n1_pred) n2) (bite (if_z n2)
+                                                      voidtp
+                                                      (leq_t (app n1_pred triv)
+                                                             (app (ppi2 n2) triv))).
+  intros.
+  unfold leq_t. unfold wind.
+  eapply equiv_trans.
+  {
+    apply equiv_app.
+    { apply equiv_app.
+      { apply steps_equiv. apply theta_fix. }
+      {apply equiv_refl. }
+    }
+    {apply equiv_refl. }
+  }
+  {
+  eapply equiv_trans.
+  {
+    apply equiv_app.
+    { apply equiv_app.
+      { apply reduce_equiv. apply reduce_app_beta; apply reduce_id.
+      }
+      {apply equiv_refl. }
+    }
+    {apply equiv_refl. }
+  }
+  {
+    simpsub. simpl. simpsub.
+    eapply equiv_trans.
+  {
+    apply equiv_app.
+    { apply reduce_equiv. apply reduce_app_beta; apply reduce_id.
+      }
+      {apply equiv_refl. }
+    }
+  { simpsub. simpl.
+    eapply equiv_trans.
+    {
+      apply equiv_app.
+      {
+        apply equiv_app.
+        {
+          apply equiv_app.
+          {
+            apply reduce_equiv. apply reduce_app_beta. apply reduce_id.
+            unfold nzero. apply reduce_ppi1_beta. apply reduce_id.
+          }
+          {
+            unfold nsucc. apply reduce_equiv. apply reduce_ppi2_beta. apply reduce_id.
+          }
+        }
+        apply equiv_refl.
+      }
+      {apply equiv_refl. }
+    }
+    { simpsub. simpl.
+    eapply equiv_trans.
+    {
+      apply equiv_app.
+      {
+        apply equiv_app.
+        {
+          apply reduce_equiv. apply reduce_app_beta; apply reduce_id.
+        }
+        { apply equiv_refl.
+        }
+      }
+      {apply equiv_refl. }
+    }
+    { simpsub. simpl.
+      eapply equiv_trans.
+      { apply equiv_app.
+        apply reduce_equiv. apply reduce_app_beta.
+        apply reduce_bite_beta2. apply reduce_id.
+        apply reduce_id.
+        {apply equiv_refl. }
+      }
+      {
+        simpsub.
+        simpl.
+        {eapply equiv_trans.
+         { apply reduce_equiv.
+           apply reduce_app_beta; apply reduce_id. }
+           {
+             simpsub. simpl.
+             apply equiv_bite.
+             - apply equiv_refl.
+             - apply equiv_refl.
+             - apply equiv_app.
+               { eapply equiv_trans. 
+                 { apply reduce_equiv. apply reduce_app_beta;
+                   apply reduce_id. (*?*)
+                 }
+                 {simpsub. simpl.
+                  apply equiv_app.
+                  - apply equiv_refl.
+                  - unfold nsucc.
+                    apply equiv_app.
+                    apply reduce_equiv. apply reduce_ppi2_beta;
+                                          apply reduce_id. apply equiv_refl. }
+               }
+               apply equiv_refl.
+           }
+           } } } } } } }
+Qed.
+
+Lemma leq_zero_equiv n2: equiv (leq_t nzero n2) unittp. 
+  unfold leq_t. unfold wind.
+  eapply equiv_trans.
+  {
+    apply equiv_app.
+    { apply equiv_app.
+      { apply steps_equiv. apply theta_fix. }
+      {apply equiv_refl. }
+    }
+    {apply equiv_refl. }
+  }
+  {
+  eapply equiv_trans.
+  {
+    apply equiv_app.
+    { apply equiv_app.
+      { apply reduce_equiv. apply reduce_app_beta; apply reduce_id.
+      }
+      {apply equiv_refl. }
+    }
+    {apply equiv_refl. }
+  }
+  {
+    simpsub. simpl. simpsub.
+    eapply equiv_trans.
+  {
+    apply equiv_app.
+    { apply reduce_equiv. apply reduce_app_beta; apply reduce_id.
+      }
+      {apply equiv_refl. }
+    }
+  { simpsub. simpl.
+    eapply equiv_trans.
+    {
+      apply equiv_app.
+      {
+        apply equiv_app.
+        {
+          apply equiv_app.
+          {
+            apply reduce_equiv. apply reduce_app_beta. apply reduce_id.
+            unfold nzero. apply reduce_ppi1_beta. apply reduce_id.
+          }
+          {
+            unfold nzero. apply reduce_equiv. apply reduce_ppi2_beta. apply reduce_id.
+          }
+        }
+        apply equiv_refl.
+      }
+      {apply equiv_refl. }
+    }
+    { simpsub. simpl.
+    eapply equiv_trans.
+    {
+      apply equiv_app.
+      {
+        apply equiv_app.
+        {
+          apply reduce_equiv. apply reduce_app_beta; apply reduce_id.
+        }
+        { apply equiv_refl.
+        }
+      }
+      {apply equiv_refl. }
+    }
+    { simpsub. simpl.
+      eapply equiv_trans.
+      { apply equiv_app.
+        apply reduce_equiv. apply reduce_app_beta.
+        apply reduce_bite_beta1. apply reduce_id.
+        apply reduce_id.
+        {apply equiv_refl. }
+      }
+      {
+        simpsub. unfold if_z. apply reduce_equiv.
+        change unittp with (subst1 n2 unittp).
+        apply reduce_app_beta; apply reduce_id.
+      }
+    }
+    }
+    
+  }
+  }
+  }
+  Qed.
+
+
+
+
+Lemma leq_succsucc_equiv n1_pred n2_pred : equiv (leq_t (ppair bfalse n1_pred)
+                                            (ppair bfalse n2_pred))                                                                               (leq_t (app n1_pred triv)
+                                                             (app n2_pred triv)).
+  eapply equiv_trans.
+  apply leq_succ_equiv.
+  eapply equiv_trans.
+  {apply equiv_bite.
+   apply reduce_equiv. apply reduce_ppi1_beta. apply reduce_id.
+   apply equiv_refl.
+   apply equiv_app. apply equiv_refl. apply equiv_app.
+   apply reduce_equiv. apply reduce_ppi2_beta. apply reduce_id. apply equiv_refl.
+  }
+  {apply reduce_equiv. apply reduce_bite_beta2. apply reduce_id. }
+  Qed.
+
+
+Lemma leqb_succ_equiv n1_pred n2 : equiv (leqb_app (ppair bfalse n1_pred) n2) (bite (if_z n2)
+                                                     bfalse
+                                                      (leqb_app (app n1_pred triv)
+                                                                (app (ppi2 n2) triv))).
+
+  intros.
+  unfold leq_b. unfold wind.
+  eapply equiv_trans.
+  {
+    apply equiv_app.
+    { apply equiv_app.
+      { apply steps_equiv. apply theta_fix. }
+      {apply equiv_refl. }
+    }
+    {apply equiv_refl. }
+  }
+  {
+  eapply equiv_trans.
+  {
+    apply equiv_app.
+    { apply equiv_app.
+      { apply reduce_equiv. apply reduce_app_beta; apply reduce_id.
+      }
+      {apply equiv_refl. }
+    }
+    {apply equiv_refl. }
+  }
+  {
+    simpsub. simpl. simpsub.
+    eapply equiv_trans.
+  {
+    apply equiv_app.
+    { apply reduce_equiv. apply reduce_app_beta; apply reduce_id.
+      }
+      {apply equiv_refl. }
+    }
+  { simpsub. simpl.
+    eapply equiv_trans.
+    {
+      apply equiv_app.
+      {
+        apply equiv_app.
+        {
+          apply equiv_app.
+          {
+            apply reduce_equiv. apply reduce_app_beta. apply reduce_id.
+            unfold nzero. apply reduce_ppi1_beta. apply reduce_id.
+          }
+          {
+            unfold nsucc. apply reduce_equiv. apply reduce_ppi2_beta. apply reduce_id.
+          }
+        }
+        apply equiv_refl.
+      }
+      {apply equiv_refl. }
+    }
+    { simpsub. simpl.
+    eapply equiv_trans.
+    {
+      apply equiv_app.
+      {
+        apply equiv_app.
+        {
+          apply reduce_equiv. apply reduce_app_beta; apply reduce_id.
+        }
+        { apply equiv_refl.
+        }
+      }
+      {apply equiv_refl. }
+    }
+    { simpsub. simpl.
+      eapply equiv_trans.
+      { apply equiv_app.
+        apply reduce_equiv. apply reduce_app_beta.
+        apply reduce_bite_beta2. apply reduce_id.
+        apply reduce_id.
+        {apply equiv_refl. }
+      }
+      {
+        simpsub.
+        simpl.
+        {eapply equiv_trans.
+         { apply reduce_equiv.
+           apply reduce_app_beta; apply reduce_id. }
+           {
+             simpsub. simpl.
+             apply equiv_bite.
+             - apply equiv_refl.
+             - apply equiv_refl.
+             - apply equiv_app.
+               { eapply equiv_trans. 
+                 { apply reduce_equiv. apply reduce_app_beta;
+                   apply reduce_id. (*?*)
+                 }
+                 {simpsub. simpl.
+                  apply equiv_app.
+                  - apply equiv_refl.
+                  - unfold nsucc.
+                    eapply equiv_trans.
+                    apply equiv_app.
+                    apply reduce_equiv. apply reduce_ppi2_beta;
+                                          apply reduce_id. apply equiv_refl.
+                    apply equiv_refl.                  }
+               }
+               apply equiv_refl.
+           }
+           } } } } } } }
+Qed.
+
+
+
+Lemma leqb_zero_equiv n2: equiv (leqb_app nzero n2) btrue. 
+  unfold leq_b. unfold wind.
+  eapply equiv_trans.
+  {
+    apply equiv_app.
+    { apply equiv_app.
+      { apply steps_equiv. apply theta_fix. }
+      {apply equiv_refl. }
+    }
+    {apply equiv_refl. }
+  }
+  {
+  eapply equiv_trans.
+  {
+    apply equiv_app.
+    { apply equiv_app.
+      { apply reduce_equiv. apply reduce_app_beta; apply reduce_id.
+      }
+      {apply equiv_refl. }
+    }
+    {apply equiv_refl. }
+  }
+  {
+    simpsub. simpl. simpsub.
+    eapply equiv_trans.
+  {
+    apply equiv_app.
+    { apply reduce_equiv. apply reduce_app_beta; apply reduce_id.
+      }
+      {apply equiv_refl. }
+    }
+  { simpsub. simpl.
+    eapply equiv_trans.
+    {
+      apply equiv_app.
+      {
+        apply equiv_app.
+        {
+          apply equiv_app.
+          {
+            apply reduce_equiv. apply reduce_app_beta. apply reduce_id.
+            unfold nzero. apply reduce_ppi1_beta. apply reduce_id.
+          }
+          {
+            unfold nzero. apply reduce_equiv. apply reduce_ppi2_beta. apply reduce_id.
+          }
+        }
+        apply equiv_refl.
+      }
+      {apply equiv_refl. }
+    }
+    { simpsub. simpl.
+    eapply equiv_trans.
+    {
+      apply equiv_app.
+      {
+        apply equiv_app.
+        {
+          apply reduce_equiv. apply reduce_app_beta; apply reduce_id.
+        }
+        { apply equiv_refl.
+        }
+      }
+      {apply equiv_refl. }
+    }
+    { simpsub. simpl.
+      eapply equiv_trans.
+      { apply equiv_app.
+        apply reduce_equiv. apply reduce_app_beta.
+        apply reduce_bite_beta1. apply reduce_id.
+        apply reduce_id.
+        {apply equiv_refl. }
+      }
+      {
+        simpsub. unfold if_z. apply reduce_equiv.
+        change btrue with (subst1 n2 (btrue)).
+        apply reduce_app_beta; apply reduce_id.
+      }
+    }
+    }
+    
+  }
+  }
+  }
+  Qed.
